option state

lean/incorrectness_lovic_lib.lean
@@ -1,11 +1,56 @@
+import algebra
+import data.real.basic
+import data.vector
+import tactic.explode
+import tactic.find
+import tactic.induction
+import tactic.linarith
+import tactic.rcases
+import tactic.rewrite
+import tactic.ring_exp
+import tactic.tidy
+import tactic.where
 
 /-! # Incorrectness logic library -/
 
-/-! ## Language -/
-
 namespace IncLoLib
 
+meta def tactic.dec_trivial := `[exact dec_trivial]
+
+/-! ## State-/
+
 def state : Type := string -> ℕ
+
+def state.update : string -> ℕ -> state -> state
+| name val s          := (λname', if name' = name then val else s name')
+
+notation s `{` name ` ↦ ` val `}` := state.update name val s
+
+@[simp] lemma update_apply (name : string) (val : ℕ) (s : state) :
+  s{name ↦ val} name = val :=
+begin
+  calc s{name ↦ val} name = (λname', if name' = name then val else s name') name : by refl
+       ...                = val : by finish,
+end
+
+
+@[simp] lemma update_apply_ne (name name' : string) (val : ℕ) (s : state)
+    (h : name' ≠ name . tactic.dec_trivial) :
+    s{name ↦ val} name' = s name' :=
+begin
+  calc s{name ↦ val} name' = (λname', if name' = name then val else s name') name' : by refl
+       ...                 = s name' : by finish[h],
+end
+
+@[simp] lemma update_override (name : string) (val₁ val₂ : ℕ) (s : state) :
+  s{name ↦ val₂}{name ↦ val₁} = s{name ↦ val₁} :=
+begin
+  apply funext,
+  intro name',
+  by_cases name' = name; simp [h]
+end
+
+/-! ## Language -/
 
 inductive stmt : Type
 | skip   : stmt
@@ -14,17 +59,64 @@ inductive stmt : Type
 -- | ite    : (state → Prop) → stmt → stmt → stmt
 -- | while  : (state → Prop) → stmt → stmt
 
-def eval : state -> stmt -> state
-| st stmt.skip            := st
-| st (stmt.assign v s)    := λ x, if x = v then s st else st v
-| st (stmt.seq n m)       := λ x, (eval (eval st n) m) x
+def eval : option state -> stmt -> option state
+| st stmt.skip                  := st
+| none (stmt.assign v s)        := none
+| (some st) (stmt.assign v s)   := st{v ↦ s st}
+| st (stmt.seq n m)             := (eval (eval st n) m)
 
 infixr ` ;; ` : 90 := stmt.seq
 
-#eval eval (λ x, 0) stmt.skip "x"
-#eval eval (λ x, if x = "y" then 2 else 0) (stmt.assign "x" (λ s, 1 + s "y")) "x"
-#eval eval (λ x, if x = "y" then 2 else 0) 
+#eval option.bind (eval (some (λ x, 0)) stmt.skip) (λ s, some (s "x"))
+#eval option.bind (eval (some (λ x, if x = "y" then 2 else 0)) (stmt.assign "x" (λ s, 1 + s "y"))) 
+  (λ s, some (s "x"))
+#eval option.bind (eval (some (λ x, if x = "y" then 2 else 0))
   ((stmt.assign "x" (λ s, 1 + s "y")) ;; 
-   (stmt.assign "x" (λ s, 1 + s "x"))) "x"
+   (stmt.assign "x" (λ s, 1 + s "x")))) (λ s, some (s "x"))
+
+#eval option.bind (eval (none)
+  ((stmt.assign "x" (λ s, 1 + s "y")) ;; 
+   (stmt.assign "x" (λ s, 1 + s "x")))) (λ s, some (s "x"))
+
+/-! ## Big step semantics -/
+
+inductive big_step : stmt × option state → option state → Prop
+| skip {s} :
+  big_step (stmt.skip, s) s
+| assign {x f s} :
+  big_step (stmt.assign x f, some s) (some (s{x ↦ f s}))
+| seq {S T s t u} (hS : big_step (S, s) t)
+    (hT : big_step (T, t) u) :
+  big_step (S ;; T, s) u
+-- | ite_true {b : state → Prop} {S T s t} (hcond : b s)
+--     (hbody : big_step (S, s) t) :
+--   big_step (stmt.ite b S T, s) t
+-- | ite_false {b : state → Prop} {S T s t} (hcond : ¬ b s)
+--     (hbody : big_step (T, s) t) :
+--   big_step (stmt.ite b S T, s) t
+-- | while_true {b : state → Prop} {S s t u} (hcond : b s)
+--     (hbody : big_step (S, s) t)
+--     (hrest : big_step (stmt.while b S, t) u) :
+--   big_step (stmt.while b S, s) u
+-- | while_false {b : state → Prop} {S s} (hcond : ¬ b s) :
+--   big_step (stmt.while b S, s) s
+
+infix ` ⟹ ` : 110 := big_step
+
+/-! ## Hoare Logic -/
+
+def partial_hoare (P : option state → Prop) (S : stmt)
+  (Q : option state → Prop) : Prop := 
+  ∀ s t, (P s → (S, s) ⟹ t) → Q t
+
+notation `{* ` P : 1 ` *} ` S : 1 ` {* ` Q : 1 ` *}` :=
+  partial_hoare
+
+namespace hoare_logic
+
+
+
+end hoare_logic
+
 
 end IncLoLib
